Freigen.lean
@@ -1,8 +1,6 @@
 -- This module serves as the root of the `Freigen` library.
-import Freigen.Effect
-import Freigen.Tp
-import Freigen.ITree
 import Freigen.Free
+import Freigen.ITree
+import Freigen.Ast
 import Freigen.Reflect
-import Freigen.Recursion
 import Freigen.Examples
